{
 "cells": [
  {
   "cell_type": "markdown",
   "metadata": {},
   "source": [
    "__Estimators__\n",
    "\n",
    "$X$ i.i.d. $(x_1, x_2, \\ldots, x_n) = x$\n",
    "\n",
    "Let $\\theta$ be a parameter of $x$, (e.g. $\\theta=\\mathbb{E}X$, or $\\theta=VarX$)\n",
    "\n",
    "Consider function $\\hat{\\theta}(x)$\n",
    "\n",
    "which values are estimates (point) for $\\theta$\n",
    "\n",
    "Example: \n",
    "\n",
    "1) $\\theta = \\mathbb{E}X, \\hat{\\theta}(x)=\\bar{x}$\n",
    "\n",
    "2) $\\theta = Var X, \\hat{\\theta}_1 = Var(X)$ sample variance, $\\hat{\\theta}_2(x) = Var_+(x)$\n"
   ]
  },
  {
   "cell_type": "markdown",
   "metadata": {},
   "source": [
    "__Properties of estimators__\n",
    "\n",
    "1. Consistency\n",
    "\n",
    "$\\hat{\\theta}(x) \\to \\theta$ as $n \\to 0$\n",
    "\n",
    "2. Unbiasedness\n",
    "\n",
    "$\\mathbb{E}\\hat{\\theta}(x) = \\theta$ for fixed $n$\n",
    "\n",
    "example: \n",
    "\n",
    "1)\n",
    "\n",
    "$\\bar{x} \\to \\mathbb{E}X$ as $n \\to \\infty$ law of large numbers\n",
    "\n",
    "$\\implies \\bar{x}$ is consistent estimator for $\\mathbb{E}X$  \n",
    "\n",
    "---\n",
    "\n",
    "$\\mathbb{E}\\bar{x} = \\mathbb{E}X$\n",
    "\n",
    "$\\implies \\bar{x}$ is unbiased estimator for $\\mathbb{E}X$  \n",
    " \n",
    "2)\n",
    "\n",
    "Consider $\\bar{\\theta}(x) = \\frac{n}{n+1}\\bar{x}$\n",
    "\n",
    "consistent but biased: $\\mathbb{E}\\frac{n}{n+1}\\bar{x} = \\frac{n}{n+1}\\mathbb{E}\\bar{x} = \\frac{n}{n+1}\\mathbb{E}X$"
   ]
  },
  {
   "cell_type": "markdown",
   "metadata": {},
   "source": [
    "Assume that $(x_1, \\ldots, x_n)$ is i.i.d. sample from random variable $X$ with finite variance. It is known that unbiased sample variance $\\mathrm{\\mathop{Var}}_+(x)=\\frac{1}{n-1}\\sum_{i=1}^n (x_n - \\bar x)^2$ is unbiased estimator for population variance $\\mathrm{\\mathop{Var}}(X)$. Sample standard deviation is usually defined as square root of unbiased sample variance: $\\mathrm{\\mathop{SD}}(x)=\\sqrt{\\mathrm{\\mathop{Var}}_+(x)}$. Population standard deviation is square root of population variance: $\\mathrm{\\mathop{SD}}(X)=\\sqrt{\\mathrm{\\mathop{Var}}(X)}$. It is natural to ask: is it true that sample standard deviation is unbiased estimator for population standard deviation?\n",
    "\n",
    "To answer this question let us consider a simple example. Assume that $X$ is Bernoulli random variable that takes values 0 and 1 with probability $1/2$. Let $n=2$, so our sample is just $x=(x_1, x_2)$.\n",
    "\n",
    "First of all, let us find population variance, i.e. variance of X. Enter ordinary fraction.\n",
    "\n",
    "$VarX = pq = 1/4$\n",
    "\n",
    "---\n",
    "\n",
    "Now let us consider unbiased sample variance. It is a function of a sample, sample is a random variable, so unbiased sample variance is random variable as well. Let us find its distribution. It is easy to see that it can take only values 0 and $1/2$. What is the probability to take value $1/2$? Enter ordinary fraction.\n",
    "\n",
    "sample variance is: squared sum / (n-1) \n",
    "\n",
    "$((1-1/2)^2 + (0-1/2)^2) / (2-1) = 1/2 $\n",
    "\n",
    "this value is taken in case that our sample is either (1, 0), or (0, 1). Otherwise it's 0.\n",
    "\n",
    "---\n",
    "What is the expected value of unbiased sample variance?\n",
    "\n",
    "$E(Var_+X) = 1/2 * 1/2 + 1/2 * 0 = 1/4$\n",
    "\n",
    "it equals to the population variance. That's not surprising: unbiased sample variance is unbiased estimator for population variance after all!\n",
    "\n",
    "---\n",
    "\n",
    "So we see that unbiased sample variance is indeed unbiased estimator for population variance. What about standard deviation? First of all, found standard deviation of $X$. Enter ordinary fraction.\n",
    "\n",
    "$\\sqrt{1/4} = 1/2$\n",
    "\n",
    "---\n",
    "Now let us consider sample standard deviation. Again, it is a function of sample and therefore is random variable. Let's find its distribution. We know that the only non-zero value that unbiased sample variance can take in our example is 1/2. It follows that the only non-zero value that sample standard deviation can take is $\\sqrt{1/2}$. What is the probability to take this value?\n",
    "\n",
    "1/2\n",
    "\n",
    "if unbiased sample variance takes value 1/2, then sample standard deviation takes value $\\sqrt{1/2}$. And this probability already known.\n",
    "\n",
    "---\n",
    "Now find expected value of sample standard deviation. \n",
    "\n",
    "$1/2 \\times \\sqrt{1/2} + 1/2 \\times 0 = 1/(2\\sqrt{2})$\n",
    "\n",
    "---\n",
    "\n",
    "Now we are ready to answer the question: is sample standard deviation unbiased estimator for population standard deviation?\n",
    "\n",
    "expected value of sample standard deviation. $\\ne$ standard deviation of $X$\n",
    "\n",
    "$1/2 \\ne 1/(2\\sqrt{2})$"
   ]
  },
  {
   "cell_type": "markdown",
   "metadata": {},
   "source": [
    "Let $x=(x_1, \\ldots, x_n)$ be i.i.d. sample from some random variable XX with finite variance. Prove that:\n",
    "\n",
    "- Biased sample variance $\\mathrm{\\mathop{Var}}(x)=\\frac{1}{n}\\sum_{i=1}^n(x_i-\\bar x)^2$ is biased estimator for population variance (i.e. $\\mathrm{\\mathop{Var}}(X)$)\n",
    "- Unbiased sample variance $\\mathrm{\\mathop{Var_+}}(x)=\\frac{1}{n-1}\\sum_{i=1}^n(x_i-\\bar x)^2$ is consistencent and unbiased sample variance.\n",
    "\n",
    "You have to use definition of variance, properties of expected value and some algebra. It is easier to begin with the case \\mathbb EX=0EX=0 and expand the expression under the sum."
   ]
  },
  {
   "cell_type": "markdown",
   "metadata": {},
   "source": [
    "$\\bar{x} = \\frac{1}{n} \\sum^n_{i=1}x_i$\n",
    "\n",
    "$Var(x_i) = \\sigma^2$\n",
    "\n",
    "$Var(\\bar{x}) = Var(\\frac{x_1 + x_2 + \\ldots + x_n}{n}) = Var(\\frac{x_1}{n} + \\frac{x_2}{n} + \\dots + \\frac{x_n}{n}) = \\frac{1}{n^2}(Var(x_1) + Var(x_2) + \\dots + Var(x_n)) = \\frac{1}{n^2} n\\sigma^2 = \\frac{\\sigma^2}{n}$\n",
    "\n",
    "$\\sum^n_{i=1}(x_i-\\bar{x})^2 = \\sum^n_{i=1}(x_i^2 - 2\\bar{x}x_i + \\bar{x}^2)$  \n",
    "$= \\sum^n_{i=1} x_i^2 - 2 \\bar{x} \\sum^n_{i=1} x_i + \\sum^n_{i=1} \\bar{x}^2$  \n",
    "$= \\sum^n_{i=1} x_i^2 - 2 n \\bar{x}^2 + n \\bar{x}^2$  \n",
    "$= \\sum^n_{i=1} x_i^2 - n \\bar{x}^2$\n",
    "\n",
    "$\\mathbb{E}(\\sum^n_{i=1}(x_i-\\bar{x})^2)$  \n",
    "$= \\mathbb{E}(\\sum^n_{i=1}((x_i - \\mu) - (\\bar{x} - \\mu))^2)$  \n",
    "$= \\mathbb{E}(\\sum^n_{i=1}(x_i - \\mu)^2 - n(\\bar{x} - \\mu)^2)$  \n",
    "$= \\sum^n_{i=1}\\mathbb{E}(x_i - \\mu)^2 - n\\mathbb{E}(\\bar{x} - \\mu)^2$  \n",
    "$= \\sum^n_{i=1}Var(x_i) - nVar(\\bar{x})$  \n",
    "$= \\sum^n_{i=1}\\sigma^2 - \\sigma^2$  \n",
    "$= n\\sigma^2 - \\sigma^2$  \n",
    "\n",
    "$\\mathbb{E}(Var(x)) = \\mathbb{E}( \\frac{1}{n}\\sum^n_{i=1}(x_i-\\bar{x})^2 )$\n",
    "$\\frac{1}{n} (n\\sigma^2 - \\sigma^2) = \\frac{n-1}{n} \\sigma^2$\n",
    "\n",
    "$\\mathbb{E}(Var_+(x)) = \\mathbb{E}( \\frac{1}{n-1}\\sum^n_{i=1}(x_i-\\bar{x})^2 )$\n",
    "$\\frac{1}{n-1} (n\\sigma^2 - \\sigma^2) = \\sigma^2$"
   ]
  }
 ],
 "metadata": {
  "kernelspec": {
   "display_name": "Python 3",
   "language": "python",
   "name": "python3"
  },
  "language_info": {
   "codemirror_mode": {
    "name": "ipython",
    "version": 3
   },
   "file_extension": ".py",
   "mimetype": "text/x-python",
   "name": "python",
   "nbconvert_exporter": "python",
   "pygments_lexer": "ipython3",
   "version": "3.7.9"
  }
 },
 "nbformat": 4,
 "nbformat_minor": 4
}
